bin_prelims.v
@@ -12,12 +12,18 @@ Open Scope N_scope.
 
 (*
 =============================================================================
-****************** SECTION 1: PRELIMINARIES *********************************
+***************** SECTION 8: BINARY PRELIMINARIES ***************************
 =============================================================================
  *)
 
-(* This file contains recurrently useful results and definitions
-   that are used throughout the subsequent files *)
+(* The files named "bin_" constitue a parallel development of our
+ * techniques, working in Coq's binary type N, as described in Section 6.
+ *)
+
+(* 
+ * This file contains recurrently useful results and definitions
+ * that are used throughout the subsequent files 
+ *)
 
 Lemma le_antisym: forall m n : N, (m <= n) -> (n <= m) -> (m = n).
 Proof. intros. lia. Qed.
@@ -51,7 +57,8 @@ Qed.
 Lemma le_div_mul : forall a b q : N, b <> 0 -> (q <= a / b) <-> (b * q <= a).
 Proof.
   intros a b q Hb. split; intro H.
-  - rewrite N.le_ngt. intro contra. apply N.div_lt_upper_bound in contra; [lia|trivial].
+  - rewrite N.le_ngt. intro contra.
+    apply N.div_lt_upper_bound in contra; [lia | trivial].
   - apply N.div_le_lower_bound; trivial.
 Qed.
 
@@ -59,7 +66,7 @@ Lemma div_sub : forall a b c, c <> 0 -> (a - c * b) / c = a / c - b.
 Proof.
   intros a b c Hc. destruct (N.le_gt_cases a (c * b)) as [H|H].
   - replace (a / c - b) with 0 by
-      (symmetry; rewrite N.sub_0_le; apply N.div_le_upper_bound; trivial).
+        (symmetry; rewrite N.sub_0_le; apply N.div_le_upper_bound; trivial).
     rewrite <- N.sub_0_le in H. rewrite H. apply N.div_0_l, Hc.
   - replace a with (a - c * b + b * c) at 2 by lia.
     rewrite N.div_add by trivial. lia.
@@ -74,18 +81,18 @@ Fixpoint repeat (f: N -> N) (rep : nat) (n : N) : N :=
   end.
 
 Theorem repeat_S_comm :
-    forall f k n, repeat f (S k) n = repeat f k (f n).
+  forall f k n, repeat f (S k) n = repeat f k (f n).
 Proof.
   induction k; trivial. intro. simpl in *. rewrite IHk. trivial.
 Qed.
 
 Theorem repeat_plus :
-    forall f k l n, repeat f (k + l) n = repeat f k (repeat f l n).
+  forall f k l n, repeat f (k + l) n = repeat f k (repeat f l n).
 Proof. induction k; trivial. simpl; intros; rewrite IHk; trivial. Qed.
 
+
 (* ****** INCREASING FUNCTIONS ****** *)
-Definition increasing (f : N -> N) : Prop :=
-  forall n m, n < m -> f n < f m.
+Definition increasing (f : N -> N) : Prop := forall n m, n < m -> f n < f m.
 
 
 (* ****** NAT_SIZE ************ *)
@@ -98,26 +105,26 @@ Definition nat_size (n : N) : nat :=
                   match x with
                   | xH => 1%nat
                   | xI y | xO y => S (nat_pos_size y) end
-                  in nat_pos_size p
+              in nat_pos_size p
   end.
 
 (* nat_size is increasing *)
 Lemma nat_size_incr :
-    forall m n, m <= n -> (nat_size m <= nat_size n)%nat.
+  forall m n, m <= n -> (nat_size m <= nat_size n)%nat.
 Proof.
   intros m n Hmn.
   destruct m as [|pm]. simpl. omega.
   destruct n as [|pn]. lia.
   generalize dependent pm.
   induction pn;
-  intros; [ | |replace (Npos pm) with 1 by lia; trivial];
-  destruct pm; simpl; try omega; apply le_n_S; apply IHpn; lia.
+    intros; [ | |replace (Npos pm) with 1 by lia; trivial];
+      destruct pm; simpl; try omega; apply le_n_S; apply IHpn; lia.
 Qed.
 
 
 (* Binary contraction contracts size *)
 Lemma div2_nat_size :
-    forall m n, 0 < n -> m <= n / 2 -> (1 + nat_size m <= nat_size n)%nat.
+  forall m n, 0 < n -> m <= n / 2 -> (1 + nat_size m <= nat_size n)%nat.
 Proof.
   intros m n Hn Hmn. apply (Nat.le_trans _ (1 + nat_size (n / 2)) _).
   - apply le_n_S. apply nat_size_incr. apply Hmn.
@@ -126,7 +133,7 @@ Proof.
 Qed.
 
 Lemma div2_contr :
-    forall m n, 0 < n -> m <= n / 2 -> m < n.
+  forall m n, 0 < n -> m <= n / 2 -> m < n.
 Proof.
   intros m n Hn Hmn. apply (div2_nat_size m n Hn) in Hmn.
   rewrite N.lt_nge. intro. apply nat_size_incr in H. omega.
@@ -158,7 +165,8 @@ Lemma to_N_func_repeat : forall f k,
     repeat f k = to_N_func (prelims.repeat (to_nat_func f) k).
 Proof.
   intros f k. induction k; apply functional_extensionality;
-  intro n; simpl; unfold to_N_func; [symmetry; apply N2Nat.id|repeat f_equal].
+                intro n; simpl; unfold to_N_func;
+                  [symmetry; apply N2Nat.id | repeat f_equal].
   rewrite IHk. unfold to_nat_func. rewrite N2Nat.id. unfold to_N_func. trivial.
 Qed.
 
@@ -166,7 +174,8 @@ Lemma to_nat_func_repeat : forall f k,
     prelims.repeat f k = to_nat_func (repeat (to_N_func f) k).
 Proof.
   intros f k. induction k; apply functional_extensionality;
-  intro n; simpl; unfold to_nat_func; [symmetry; apply Nat2N.id|repeat f_equal].
+                intro n; simpl; unfold to_nat_func;
+                  [symmetry; apply Nat2N.id | repeat f_equal].
   rewrite IHk. unfold to_N_func. rewrite Nat2N.id. unfold to_nat_func. trivial.
 Qed.
 
